

ASSIGNMENT 7

5.1

Use mathematical induction in Exercises 3–17 to prove summation formulae. Be sure to identify where you use the inductive hypothesis.

3. Let $P(n)$ be the statement that $1^2 + 2^2 + \cdots + n^2 = n(n+1)(2n+1)/6$ for the positive integer n .
 - a) What is the statement $P(1)$?
 - b) Show that $P(1)$ is true, completing the basis step of the proof.
 - c) What is the inductive hypothesis?
 - d) What do you need to prove in the inductive step?
 - e) Complete the inductive step, identifying where you use the inductive hypothesis.
4. Let $P(n)$ be the statement that $1^3 + 2^3 + \cdots + n^3 = (n(n+1)/2)^2$ for the positive integer n .
 - a) What is the statement $P(1)$?
 - b) Show that $P(1)$ is true, completing the basis step of the proof.
 - c) What is the inductive hypothesis?
 - d) What do you need to prove in the inductive step?
 - e) Complete the inductive step, identifying where you use the inductive hypothesis.
5. Prove that $1^2 + 3^2 + 5^2 + \cdots + (2n+1)^2 = (n+1)(2n+1)(2n+3)/3$ whenever n is a nonnegative integer.
6. Prove that $1 \cdot 1! + 2 \cdot 2! + \cdots + n \cdot n! = (n+1)! - 1$ whenever n is a positive integer.
7. Prove that $3 + 3 \cdot 5 + 3 \cdot 5^2 + \cdots + 3 \cdot 5^n = 3(5^{n+1} - 1)/4$ whenever n is a nonnegative integer.
8. Prove that $2 - 2 \cdot 7 + 2 \cdot 7^2 - \cdots + 2(-7)^n = (1 - (-7)^{n+1})/4$ whenever n is a nonnegative integer.

9. a) Find a formula for the sum of the first n even positive integers.
 b) Prove the formula that you conjectured in part (a).
10. a) Find a formula for

$$\frac{1}{1 \cdot 2} + \frac{1}{2 \cdot 3} + \cdots + \frac{1}{n(n+1)}$$

by examining the values of this expression for small values of n .

- b) Prove the formula you conjectured in part (a).
11. a) Find a formula for

$$\frac{1}{2} + \frac{1}{4} + \frac{1}{8} + \cdots + \frac{1}{2^n}$$

by examining the values of this expression for small values of n .

- b) Prove the formula you conjectured in part (a).
12. Prove that

$$\sum_{j=0}^n \left(-\frac{1}{2}\right)^j = \frac{2^{n+1} + (-1)^n}{3 \cdot 2^n}$$

whenever n is a nonnegative integer.

13. Prove that $1^2 - 2^2 + 3^2 - \cdots + (-1)^{n-1}n^2 = (-1)^{n-1}n(n+1)/2$ whenever n is a positive integer.
14. Prove that for every positive integer n , $\sum_{k=1}^n k2^k = (n-1)2^{n+1} + 2$.
15. Prove that for every positive integer n ,

$$1 \cdot 2 + 2 \cdot 3 + \cdots + n(n+1) = n(n+1)(n+2)/3.$$

16. Prove that for every positive integer n ,

$$\begin{aligned} 1 \cdot 2 \cdot 3 + 2 \cdot 3 \cdot 4 + \cdots + n(n+1)(n+2) \\ = n(n+1)(n+2)(n+3)/4. \end{aligned}$$

17. Prove that $\sum_{j=1}^n j^4 = n(n+1)(2n+1)(3n^2+3n-1)/30$ whenever n is a positive integer.

Use mathematical induction to prove the inequalities in Exercises 18–30.

18. Let $P(n)$ be the statement that $n! < n^n$, where n is an integer greater than 1.

- a) What is the statement $P(2)$?
- b) Show that $P(2)$ is true, completing the basis step of the proof.
- c) What is the inductive hypothesis?
- d) What do you need to prove in the inductive step?
- e) Complete the inductive step.

19. Let $P(n)$ be the statement that

$$1 + \frac{1}{4} + \frac{1}{9} + \cdots + \frac{1}{n^2} < 2 - \frac{1}{n},$$

where n is an integer greater than 1.

- a) What is the statement $P(2)$?
 - b) Show that $P(2)$ is true, completing the basis step of the proof.
 - c) What is the inductive hypothesis?
 - d) What do you need to prove in the inductive step?
 - e) Complete the inductive step.
20. Prove that $3^n < n!$ if n is an integer greater than 6.
21. Prove that $2^n > n^2$ if n is an integer greater than 4.
22. For which nonnegative integers n is $n^2 \leq n!$? Prove your answer.
23. For which nonnegative integers n is $2n + 3 \leq 2^n$? Prove your answer.
24. Prove that $1/(2n) \leq [1 \cdot 3 \cdot 5 \cdots (2n - 1)] / (2 \cdot 4 \cdot \cdots \cdot 2n)$ whenever n is a positive integer.

Use mathematical induction in Exercises 31–37 to prove divisibility facts.

31. Prove that 2 divides $n^2 + n$ whenever n is a positive integer.
32. Prove that 3 divides $n^3 + 2n$ whenever n is a positive integer.
33. Prove that 5 divides $n^5 - n$ whenever n is a nonnegative integer.
34. Prove that 6 divides $n^3 - n$ whenever n is a nonnegative integer.

Use mathematical induction in Exercises 38–46 to prove results about sets.

38. Prove that if A_1, A_2, \dots, A_n and B_1, B_2, \dots, B_n are sets such that $A_j \subseteq B_j$ for $j = 1, 2, \dots, n$, then

$$\bigcup_{j=1}^n A_j \subseteq \bigcup_{j=1}^n B_j.$$

39. Prove that if A_1, A_2, \dots, A_n and B_1, B_2, \dots, B_n are sets such that $A_j \subseteq B_j$ for $j = 1, 2, \dots, n$, then

$$\bigcap_{j=1}^n A_j \subseteq \bigcap_{j=1}^n B_j.$$

40. Prove that if A_1, A_2, \dots, A_n and B are sets, then

$$\begin{aligned}(A_1 \cap A_2 \cap \dots \cap A_n) \cup B \\ = (A_1 \cup B) \cap (A_2 \cup B) \cap \dots \cap (A_n \cup B).\end{aligned}$$

41. Prove that if A_1, A_2, \dots, A_n and B are sets, then

$$\begin{aligned}(A_1 \cup A_2 \cup \dots \cup A_n) \cap B \\ = (A_1 \cap B) \cup (A_2 \cap B) \cup \dots \cup (A_n \cap B).\end{aligned}$$

42. Prove that if A_1, A_2, \dots, A_n and B are sets, then

$$\begin{aligned}(A_1 - B) \cap (A_2 - B) \cap \dots \cap (A_n - B) \\ = (A_1 \cap A_2 \cap \dots \cap A_n) - B.\end{aligned}$$

43. Prove that if A_1, A_2, \dots, A_n are subsets of a universal set U , then

$$\overline{\bigcup_{k=1}^n A_k} = \bigcap_{k=1}^n \overline{A_k}.$$

5.3

- Find $f(1)$, $f(2)$, $f(3)$, and $f(4)$ if $f(n)$ is defined recursively by $f(0) = 1$ and for $n = 0, 1, 2, \dots$
 - $f(n+1) = f(n) + 2$.
 - $f(n+1) = 3f(n)$.
 - $f(n+1) = 2^{f(n)}$.
 - $f(n+1) = f(n)^2 + f(n) + 1$.
- Find $f(1)$, $f(2)$, $f(3)$, $f(4)$, and $f(5)$ if $f(n)$ is defined recursively by $f(0) = 3$ and for $n = 0, 1, 2, \dots$
 - $f(n+1) = -2f(n)$.
 - $f(n+1) = 3f(n) + 7$.
 - $f(n+1) = f(n)^2 - 2f(n) - 2$.
 - $f(n+1) = 3^{f(n)/3}$.
- Find $f(2)$, $f(3)$, $f(4)$, and $f(5)$ if f is defined recursively by $f(0) = -1$, $f(1) = 2$, and for $n = 1, 2, \dots$
 - $f(n+1) = f(n) + 3f(n-1)$.
 - $f(n+1) = f(n)^2 f(n-1)$.
 - $f(n+1) = 3f(n)^2 - 4f(n-1)^2$.
 - $f(n+1) = f(n-1)/f(n)$.
- Find $f(2)$, $f(3)$, $f(4)$, and $f(5)$ if f is defined recursively by $f(0) = f(1) = 1$ and for $n = 1, 2, \dots$
 - $f(n+1) = f(n) - f(n-1)$.
 - $f(n+1) = f(n)f(n-1)$.
 - $f(n+1) = f(n)^2 + f(n-1)^3$.
 - $f(n+1) = f(n)/f(n-1)$.
- Determine whether each of these proposed definitions is a valid recursive definition of a function f from the set of nonnegative integers to the set of integers. If f is well defined, find a formula for $f(n)$ when n is a nonnegative integer and prove that your formula is valid.
 - $f(0) = 0$, $f(n) = 2f(n-2)$ for $n \geq 1$
 - $f(0) = 1$, $f(n) = f(n-1) - 1$ for $n \geq 1$
 - $f(0) = 2$, $f(1) = 3$, $f(n) = f(n-1) - 1$ for $n \geq 2$
 - $f(0) = 1$, $f(1) = 2$, $f(n) = 2f(n-2)$ for $n \geq 2$

6. Determine whether each of these proposed definitions is a valid recursive definition of a function f from the set of nonnegative integers to the set of integers. If f is well defined, find a formula for $f(n)$ when n is a nonnegative integer and prove that your formula is valid.
- $f(0) = 1, f(n) = -f(n-1)$ for $n \geq 1$
 - $f(0) = 1, f(1) = 0, f(2) = 2, f(n) = 2f(n-3)$ for $n \geq 3$
 - $f(0) = 0, f(1) = 1, f(n) = 2f(n+1)$ for $n \geq 2$
 - $f(0) = 0, f(1) = 1, f(n) = 2f(n-1)$ for $n \geq 1$
 - $f(0) = 2, f(n) = f(n-1)$ if n is odd and $n \geq 1$ and $f(n) = 2f(n-2)$ if $n \geq 2$
7. Give a recursive definition of the sequence $\{a_n\}$, $n = 1, 2, 3, \dots$ if
- $a_n = 6n.$
 - $a_n = 2n + 1.$
 - $a_n = 10^n.$
 - $a_n = 5.$
8. Give a recursive definition of the sequence $\{a_n\}$, $n = 1, 2, 3, \dots$ if
- $a_n = 4n - 2.$
 - $a_n = 1 + (-1)^n.$
 - $a_n = n(n+1).$
 - $a_n = n^2.$
9. Let F be the function such that $F(n)$ is the sum of the first n positive integers. Give a recursive definition of $F(n)$.

In Exercises 12–19 f_n is the n th Fibonacci number.

- Prove that $f_1^2 + f_2^2 + \dots + f_n^2 = f_n f_{n+1}$ when n is a positive integer.
- Prove that $f_1 + f_3 + \dots + f_{2n-1} = f_{2n}$ when n is a positive integer.

5.4

- Give a recursive algorithm for computing nx whenever n is a positive integer and x is an integer, using just addition.
- Give a recursive algorithm for finding the sum of the first n positive integers.
- Give a recursive algorithm for finding the sum of the first n odd positive integers.

10. Give a recursive algorithm for finding the maximum of a finite set of integers, making use of the fact that the maximum of n integers is the larger of the last integer in the list and the maximum of the first $n - 1$ integers in the list.
11. Give a recursive algorithm for finding the minimum of a finite set of integers, making use of the fact that the minimum of n integers is the smaller of the last integer in the list and the minimum of the first $n - 1$ integers in the list.
17. Describe a recursive algorithm for multiplying two non-negative integers x and y based on the fact that $xy = 2(x \cdot (y/2))$ when y is even and $xy = 2(x \cdot \lfloor y/2 \rfloor) + x$ when y is odd, together with the initial condition $xy = 0$ when $y = 0$.
23. Devise a recursive algorithm for computing n^2 where n is a nonnegative integer, using the fact that $(n + 1)^2 = n^2 + 2n + 1$. Then prove that this algorithm is correct.
24. Devise a recursive algorithm to find a^{2^n} , where a is a real number and n is a positive integer. [*Hint:* Use the equality $a^{2^{n+1}} = (a^{2^n})^2$.]

A. (Group Assignment) Do and submit:

5.1: 3, 7, 11, 19, 21, 31, 33, 39, 41.

5.3: 3, 5, 7.

B. (Individual Coding Assignment) Deadline for submitting code:

Code: 10 algorithms in Section 5.4 (slide) + 5.4: 7-11, 17, 23, 24.